src/Appraisal_AltImpls_Eq.v
@@ -21,7 +21,7 @@ Set Nested Proofs Allowed.
 Lemma appraisal_alt : forall ec1 ec2 ec2' ls et,
 
   Some ec1 = Impl_appraisal_alt.build_app_comp_evC et ls ->
-  Some ec2 = reconstruct_ev (evc ls et) ->
+  reconstruct_evP (evc ls et) ec2 ->
   ec2' = Impl_appraisal.build_app_comp_evC ec2 ->
   ec1 = ec2'.
 Proof.
@@ -29,22 +29,30 @@ Proof.
   generalizeEverythingElse ec2.
   induction ec2; intros.
   -
+    do_inv_recon.
     ff.
+    (*
     subst.
     assert (et = mt).
     { eapply inv_recon_mt; eauto. }
     subst.
-    ff.
+    ff. *)
   -
+    do_inv_recon.
+    (*
     ff.
     subst.
     assert (et = nn n).
     { eapply inv_recon_nn; eauto. }
     subst.
+     *)
+    
     repeat ff.
     unfold checkNonceF.
     jkjke.
   -
+    do_inv_recon.
+    (*
     ff.
     subst.
     ff.
@@ -52,19 +60,26 @@ Proof.
     { eapply inv_recon_uu; eauto. }
     destruct_conjs.
     subst.
+     *)
+    
     repeat ff.
 
-    assert (e0 = (Impl_appraisal.build_app_comp_evC e1)).
+    assert (e = (Impl_appraisal.build_app_comp_evC ec2)).
     {
       eapply IHec2.
       jkjke.
-      jkjke.
+      invc H0.
+      repeat ff.
+      econstructor.
+      ff.
       tauto.
     }
     subst.
     unfold checkASPF.
     jkjke.
   -
+    do_inv_recon.
+    (*
     ff.
     subst.
     ff.
@@ -72,87 +87,125 @@ Proof.
     { eapply inv_recon_gg; eauto. }
     destruct_conjs.
     subst.
+     *)
+    do_recon_inv.
+    
     repeat ff.
 
-    assert (e0 = (Impl_appraisal.build_app_comp_evC e1)).
-    {
-      eapply IHec2.
-      jkjke.
-      jkjke.
-      tauto.
-    }
+    assert (e = (Impl_appraisal.build_app_comp_evC ec2)) by eauto.
     subst.
     unfold checkSig.
     unfold checkSigF.
     unfold checkSig.
-    assert (checkSigBits e n n1 =
-            checkSigBits (encodeEv e1) n n1).
+    assert (checkSigBits H2 n n0 =
+            checkSigBits (encodeEv ec2) n n0).
     {
-      assert (e = encodeEv e1).
+      assert (H2 = encodeEv ec2).
       {
         eapply recon_encodeEv.
-        2: { eassumption. }
-
-        eapply wf_recon; eauto.
+        eapply wf_recon.
+        eassumption.
+        eassumption.
       }
-      congruence.
+      subst.
+      tauto.
     }
     rewrite <- H.
-    rewrite Heqo1.
+    rewrite Heqo0.
     ff.
   -
+    do_inv_recon.
+    (*
     ff.
     subst.
     assert (et = hh n e).
     { eapply inv_recon_hh; eauto.
     }
-    subst.
+    subst. *)
     repeat ff.
     unfold checkHashF.
     jkjke.
   -
+    do_inv_recon.
+    (*
     ff.
     assert (exists et1 et2, et = ss et1 et2).
     { eapply inv_recon_ss; eauto. }
     destruct_conjs.
     subst.
+     *)
+    do_recon_inv.
+    
     repeat ff.
 
-    assert (e = (Impl_appraisal.build_app_comp_evC e1))
-           by eauto.
-
-    assert (e0 = (Impl_appraisal.build_app_comp_evC e2))
-      by eauto.
+    assert (e = (Impl_appraisal.build_app_comp_evC ec2_1)) by eauto.
+    (*
+    {
+      eapply IHec2_1.
+      symmetry.
+      eassumption.
+      invc H0.
+      repeat ff.
+      econstructor.
+      ff.
+      tauto.
+    }
+     *)
+    
+    assert (e0 = (Impl_appraisal.build_app_comp_evC ec2_2)) by eauto.
+    (*
+    {
+      eapply IHec2_2.
+      symmetry.
+      eassumption.
+      invc H0.
+      repeat ff.
+      econstructor.
+      ff.
+      tauto.
+    }
+     *)
     
     congruence.
+
   -
+    do_inv_recon.
+    (*
     ff.
-    assert (exists et1 et2, et = pp et1 et2).
-    { eapply inv_recon_pp; eauto. }
+    assert (exists et1 et2, et = ss et1 et2).
+    { eapply inv_recon_ss; eauto. }
     destruct_conjs.
     subst.
+     *)
+    do_recon_inv.
+    
     repeat ff.
 
-    assert (e = (Impl_appraisal.build_app_comp_evC e1))
-           by eauto.
-
-    assert (e0 = (Impl_appraisal.build_app_comp_evC e2))
-      by eauto.
+    assert (e = (Impl_appraisal.build_app_comp_evC ec2_1)) by eauto.
+    (*
+    {
+      eapply IHec2_1.
+      symmetry.
+      eassumption.
+      invc H0.
+      repeat ff.
+      econstructor.
+      ff.
+      tauto.
+    }
+     *)
     
+    assert (e0 = (Impl_appraisal.build_app_comp_evC ec2_2)) by eauto.
+    (*
+    {
+      eapply IHec2_2.
+      symmetry.
+      eassumption.
+      invc H0.
+      repeat ff.
+      econstructor.
+      ff.
+      tauto.
+    } *)
     congruence.
 Defined.
-
-
-(*
-    well_formed_r t ->
-    wf_ec ee ->
-    Some e' = (reconstruct_ev ecc) ->
-    copland_compile t
-                    {| st_ev := ee; st_trace := tr; st_pl := p |} =
-    (Some tt, {| st_ev := ecc;
-                 st_trace := tr';
-                 st_pl := p' |}) ->
-
-    measEvent t p (get_et ee) ev ->
-    appEvent_EvidenceC ev (build_app_comp_evC e').
-*)
